---
title: Easy calc
level: 2
flag: FLAG{Do_the_math396691ba7d7270a}
writer: Laika
---

# Easy calc

## å•é¡Œæ–‡

ðŸ˜†

## è§£æ³•
ãƒ•ãƒ©ã‚°ãŒ $s$ ã®å€¤ã‚’éµã¨ã—ã¦æš—å·åŒ–ã•ã‚Œã¦ã„ã¾ã™ã€‚
ä¸Žãˆã‚‰ã‚ŒãŸ $A := f(s, p), p$ ã®å€¤ã‹ã‚‰ $s$ ã‚’å¾©å…ƒã§ããªã„ã‹è€ƒãˆã¦ã¿ã¾ã™ã€‚
ã¾ãšã€ $A = f(s, p)$ ã®ä¸­èº«ã‚’å¼ã«èµ·ã“ã—ã¦ã¿ã¾ã™ã€‚

$$
\begin{aligned}
A = f(s, p) &= s(\dots( s(s(s(p-0)+(p-1))+(p-2)) + \dots + 2) + 1 \mod p \\\\
  &= \sum_{i=0}^{p-1} s^{p-i}(p-i) \\\\
  &= \sum_{i=1}^{p} s^{i}i 
\end{aligned}
$$

ã•ã‚‰ã«æ›¸ãä¸‹ã—ã€ $sA$ ã¨ã®å·®ã‚’è€ƒãˆã‚‹ã¨

$$
\begin{aligned}
    A &= 1 \cdot s^1 + & 2 \cdot s^2 & + \cdots + & (p-1) \cdot s^{p-1} & + & p \cdot s^{p} & \\\\
-) sA &=               & 1 \cdot s^2 & + \cdots + & (p-2) \cdot s^{p-1} & + & (p-1) \cdot s^{p} & + p \cdot s^{p+1} \\\\
(1-s)A &= 1 \cdot s^1 + & 1 \cdot s^2 & + \cdots + & 1 \cdot s^{p-1} & + & 1 \cdot s^{p} & - p \cdot s^{p+1} \\\\
       &= \frac{s(1-s^p)}{1-s} \\\\
       &= s \ \ (\because s^p = s \mod p) \\\\
\therefore \ \ s &= \frac{A}{1+A} \mod p
\end{aligned}
$$

$s$ ã‚’ $A, p$ ã®å¼ã§è¡¨ã›ãŸã®ã§ã€ã“ã‚Œã‚’éµã¨ã—ã¦AES-CBCã®æš—å·æ–‡ã‚’å¾©å·ã™ã‚Œã°ã‚ˆã„ã§ã™ã€‚

### è£œè¶³
Cryptoã§ã¯å¾€ã€…ã«ã—ã¦æ•°å¼ã‚’ã“ã­ãã‚Šå›žã™ã“ã¨ãŒã‚ã‚‹ã®ã§ã€åˆå¿ƒè€…ã®æ–¹ã«ã¯ã“ã®å·¥ç¨‹ã«æ…£ã‚Œã¦ã»ã—ã„ã¨ã„ã†æ€ã„ã§ä½œå•ã—ã¾ã—ãŸã€‚


## Solution 


The flag is encrypted using the value of $s$ as a key.
Let's consider if we can recover $s$ from the given values $A := f(s, p)$ and $p$.
First, let's express the contents of $A$ in equation form.

$$
\begin{aligned}
A = f(s, p) &= s(\dots( s(s(s(p-0)+(p-1))+(p-2)) + \dots + 2) + 1 \mod p \\\\
  &= \sum_{i=0}^{p-1} s^{p-i}(p-i) \\\\
  &= \sum_{i=1}^{p} s^{i}i 
\end{aligned}
$$

By further expanding and considering the difference with $sA$, we have

$$
\begin{aligned}
    A &= 1 \cdot s^1 + & 2 \cdot s^2 & + \cdots + & (p-1) \cdot s^{p-1} & + & p \cdot s^{p} & \\\\
-) sA &=               & 1 \cdot s^2 & + \cdots + & (p-2) \cdot s^{p-1} & + & (p-1) \cdot s^{p} & + p \cdot s^{p+1} \\\\
(1-s)A &= 1 \cdot s^1 + & 1 \cdot s^2 & + \cdots + & 1 \cdot s^{p-1} & + & 1 \cdot s^{p} & - p \cdot s^{p+1} \\\\
       &= \frac{s(1-s^p)}{1-s} \\\\
       &= s \ \ (\because s^p = s \mod p) \\\\
\therefore \ \ s &= \frac{A}{1+A} \mod p
\end{aligned}
$$

Since $s$ is expressed as a function of $A$ and $p$, we can decrypt the ciphertext encrypted with AES-CBC using this as the key.

In cryptography challenge, manipulating mathematical expressions is often required. 
This challenge was designed to help beginners get used to this kind of process.


### Solver
```python
import ast
from hashlib import md5

from Crypto.Cipher import AES
from Crypto.Util.number import *


def decrypt(ciphertext: bytes, key: int, iv: bytes) -> bytes:
    key = long_to_bytes(key)
    key = md5(key).digest()
    cipher = AES.new(key, AES.MODE_CBC, iv=iv)
    return cipher.decrypt(ciphertext)


with open("output.txt") as f:
    p = ast.literal_eval(f.readline().split("=")[1].strip())
    A = ast.literal_eval(f.readline().split("=")[1].strip())
    ciphertext = ast.literal_eval(f.readline().split("=")[1].strip())
    ciphertext = bytes.fromhex(ciphertext)


s = A * pow(1 + A, -1, p) % p
iv, ciphertext = ciphertext[:16], ciphertext[16:]
flag = decrypt(ciphertext, s, iv)
print(flag.decode())
```


